PoL/Consensus/ProtocolB/SystemB.lean
@@ -3,37 +3,26 @@ import Init.Data.Nat.Basic
 import Mathlib.Data.List.Basic
 import Mathlib.Data.List.Defs
 
-/-- A Block is represented as a string (e.g. its hash). -/
-abbrev Block := String
-
-/-- A Chain is a list of Blocks. -/
-abbrev Chain := List Block
+import PoL.Consensus.Chain
 
 /-- A Validator is modeled by its current chain and a flag indicating if it has crashed. -/
-structure Validator where
+structure ValidatorB where
     chain   : List Block
     crashed : Bool
     id      : ℕ
 deriving Repr
 
 /-- A System consists of a list of validators and a designated leader (ommitted for simplicity). -/
-structure System  where
-  validators : List Validator
+structure SystemB  where
+  validators : List ValidatorB
   leader     : ℕ
 deriving Repr
-
-/--
-Two chains are consistent if one is a prefix of the other. This ensures
-there are no forks among the chains.
--/
-def ChainsAreConsistent (c₁ c₂ : Chain) : Prop :=
-  c₁ <+: c₂ ∨ c₂ <+: c₁
 
 /--
 A system has the consistency property if the chains of any two non-crashed
 validators are consistent.
 -/
-def SystemIsConsistent (sys : System) : Prop :=
+def SystemBIsConsistent (sys : SystemB) : Prop :=
   ∀ v₁ ∈ sys.validators,
   ∀ v₂ ∈ sys.validators,
   ¬v₁.crashed → ¬v₂.crashed → ChainsAreConsistent v₁.chain v₂.chain
