PoL/Consensus/Chain.lean
@@ -1,0 +1,17 @@
+import Init.Data.Nat.Basic
+
+import Mathlib.Data.List.Basic
+import Mathlib.Data.List.Defs
+
+/-- A Block is represented as a string (e.g. its hash). -/
+abbrev Block := String
+
+/-- A Chain is a list of Blocks. -/
+abbrev Chain := List Block
+
+/--
+Two chains are consistent if one is a prefix of the other. This ensures
+there are no forks among the chains.
+-/
+def ChainsAreConsistent (c₁ c₂ : Chain) : Prop :=
+  c₁ <+: c₂ ∨ c₂ <+: c₁
